proofs/toEC/toEC_jazz.v
@@ -4,6 +4,8 @@ Require Import refresh_for.
 Require Import for_to_while.
 Require Import flatten_while.
 Require Import remove_baseop_casts.
+Require Import normalize_calls.
+Require Import make_coercions_explicit.
 
 Section TOEC.
 
@@ -17,6 +19,8 @@ Definition toEC_prog (normal : bool) (p : _uprog) : cexec _uprog :=
   Let p1 := refresh_for_prog fresh_var_ident false (normalize_cond_prog p) in
   Let p2 := if normal then for_to_while_prog fresh_var_ident p1 else ok p1 in
   let p3 := flatten_while_prog p2 in
-  remove_baseop_casts_prog fresh_var_ident p3.
+  Let p4 := remove_baseop_casts_prog fresh_var_ident p3 in
+  Let p5 := normalize_calls_prog fresh_var_ident p4 in
+  mce_prog p5.
 
 End TOEC.
